Veritas.Merkle.fst
@@ -1,6 +1,7 @@
 module Veritas.Merkle
 
 open FStar.BitVector
+open FStar.Classical
 open FStar.Seq
 open Veritas.Memory
 
@@ -47,33 +48,110 @@ let merkle_root_addr = a:merkle_addr{is_merkle_root a}
 let merkle_non_leaf_addr = a:merkle_addr{~(is_merkle_leaf a)}
 let merkle_non_root_addr = a:merkle_addr{~(is_merkle_root a)}
 
+(* Size of a hash value *)
+let hash_size = 256
+
+(* hash_value - bit vector of a specified size *)
+type hash_value = bv_t hash_size
+
+(* value stored at specific nodes of a merkle tree *)
+type merkle_payload = 
+  | MkLeaf: value:payload -> merkle_payload
+  | MkInternal: left:hash_value -> right:hash_value -> merkle_payload
+
+(* hash function maps a merkle payload to a hash value *)
+assume val hashfn (m:merkle_payload): hash_value
+
+type hash_collision = 
+  | Collision: m1:merkle_payload ->
+               m2:merkle_payload { hashfn m1 == hashfn m2 /\ ~(m1 == m2) } ->
+               hash_collision
+
 (* Traverse down a binary tree from a start node (sn) based on a bit vector *)
 let rec traverse_bin_tree (#n:pos) (b:bv_t n) (sn:bin_tree_node): Tot bin_tree_node = 
-  let child = if (index b 0) then (LeftChild sn) else (RightChild sn) in  
   if n = 1 
-  then child
+  then if index b 0 then RightChild sn else LeftChild sn
   else (
-    (* TODO: For some reason, replacing pn by (n-1) in recursive call below fails *)
-    let pn:pos = (n-1) in
-    traverse_bin_tree #pn (slice b 1 n) child)
-
-(* Map a bit vector to a binary tree node by traversing from the root *)
-let bv_to_bin_tree_node (#n:pos) (b:bv_t n): Tot bin_tree_node = traverse_bin_tree b Root
+    let tn' = traverse_bin_tree #(n-1) (slice b 0 (n-1)) sn in
+    if index b (n-1) then RightChild tn' else LeftChild tn'
+  )
 
 (* Traversing adds bit vector length to the depth *)
 let rec traverse_adds_size_to_depth (#n:pos) (b:bv_t n) (sn:bin_tree_node): 
   Lemma (requires (True))
         (ensures (depth (traverse_bin_tree b sn) = n + depth sn)) = 
-  if (n = 1) then () 
+  if (n = 1) 
+  then () 
+  else traverse_adds_size_to_depth #(n-1) (slice b 0 (n-1)) sn
+
+(* Map a bit vector to a binary tree node by traversing from the root *)
+let bv_to_bin_tree_node (#n:pos) (b:bv_t n): Tot (t:bin_tree_node{depth t = n}) = 
+  traverse_adds_size_to_depth b Root; traverse_bin_tree b Root
+
+let rec path_from_root (a:bin_tree_node{depth a > 0}): Tot (b:bv_t (depth a)) 
+  (decreases (depth a)) = 
+  if depth a = 1 
+  then (match a with
+       | LeftChild a' -> zero_vec #1
+       | RightChild a' -> ones_vec #1
+       )
+  else (match a with
+       | LeftChild a' -> (append (path_from_root a') (zero_vec #1))
+       | RightChild a' -> (append (path_from_root a') (ones_vec #1))
+       )
+
+let rec path_from_root_bv2bin_consistent_aux (#n:pos) (b:bv_t n) (i:nat{i < n}):
+  Lemma (index (path_from_root (bv_to_bin_tree_node b)) i = index b i)
+  = 
+  if n = 1 then ()  
   else (
-    let child = if (index b 0) then (LeftChild sn) else (RightChild sn) in
-    traverse_adds_size_to_depth #(n-1) (slice b 1 n) child)
+    if i = n - 1 
+    then ()
+    else path_from_root_bv2bin_consistent_aux #(n-1) (slice b 0 (n-1)) i
+  )
 
-(* Depth of the bin tree node of a bit vector is its length *)
-let bv_to_bin_tree_node_depth_is_length (#n:pos) (b:bv_t n):
-  Lemma (depth (bv_to_bin_tree_node b) = n) = 
-  traverse_adds_size_to_depth b Root
+let path_from_root_bv2bin_consistent (#n:pos) (b:bv_t n):
+  Lemma (path_from_root (bv_to_bin_tree_node b) = b) = 
+  let b' = path_from_root (bv_to_bin_tree_node b) in
+  let aux (i:nat{i < n}): Lemma ((index b' i) = (index b i)) = 
+    path_from_root_bv2bin_consistent_aux b i  
+  in
+  forall_intro aux; lemma_eq_intro b b'
 
-let merkle_leaf_addr_of_data (a:addr): Tot merkle_leaf_addr = 
-  bv_to_bin_tree_node_depth_is_length a; bv_to_bin_tree_node a
+let rec path_from_root_bv2bin_consistent2 (tn:bin_tree_node{depth tn > 0}):
+  Lemma (requires (True)) 
+        (ensures bv_to_bin_tree_node (path_from_root tn) = tn)
+  (decreases (depth tn)) =
+  let n = depth tn in
+  if n = 1 then ()
+  else match tn with 
+       | LeftChild tn' -> 
+           let p' = path_from_root tn' in
+           append_slices p' (zero_vec #1);
+           path_from_root_bv2bin_consistent2 tn'
+       | RightChild tn' -> 
+           let p' = path_from_root tn' in
+           append_slices p' (ones_vec #1);
+           path_from_root_bv2bin_consistent2 tn'
+
+(* 
+ * map each 256 bit address in memory to a leaf node of the 
+ * merkle tree
+ *)
+let addr_to_merkle_leaf (a:addr): Tot merkle_leaf_addr = 
+  bv_to_bin_tree_node a
+
+(* Inverse of addr_to_merkle_leaf *)
+let merkle_leaf_to_addr (a:merkle_leaf_addr): Tot addr = path_from_root a
+
+(*
+ * merklefn: compute the merkle tree value at each node
+ * of the merkle tree
+ *)
+let rec merklefn (a:merkle_addr) (mem: memory): Tot merkle_payload
+  (decreases (merkle_height a)) = 
+  if is_merkle_leaf a
+  then MkLeaf (mem (path_from_root a))
+  else MkInternal (hashfn (merklefn (LeftChild a) mem))
+                  (hashfn (merklefn (RightChild a) mem))
 
